\newif\ifthermosubfile
\ifdefined\THERMONOTESMAIN
  \thermosubfilefalse
\else
  \thermosubfiletrue
\fi

\providecommand{\THERMOEND}{} % safe in both modes

\ifthermosubfile
  \documentclass[11pt]{book}
  \input{./Macros/thermoHead}
  \input{./Macros/thermoSymbols}
  \graphicspath{{./Figures/}}
  \begin{document}
  \renewcommand{\THERMOEND}{\end{document}}
\fi


\chapter{ThermoS26-04}
\label{chap:ThermoS26-04}

\section{The Euler Equation}

Recall that internal energy and the entropy are homogenous of degree one:
\begin{equation}
\tilde{U}(\lambda S,\lambda V,\lambda\vec{N})=\lambda\tilde{U}(S,V,\vec{N}),\qquad \lambda>0,
\tag{3.3}\label{eq:euler-homogeneous}
\end{equation}
where
\[
\vec{N}=
\begin{bmatrix}
N_1\\
N_2\\
\vdots\\
N_r
\end{bmatrix}.
\]

\begin{theorem}
\label{thm:euler-internal-energy}
\textup{(3.1)} Let $\tilde{U}$ be the internal energy of an isolated system. Then
\begin{equation}
\tilde{U}=T S-P V+\mu_1 N_1+\cdots+\mu_r N_r.
\tag{3.4}\label{eq:euler-equation}
\end{equation}
\end{theorem}

\begin{proof}
Since $\tilde{U}$ is homogenous of degree one, differentiating \eqref{eq:euler-homogeneous} with respect to $\lambda$ we obtain
\[
T(\lambda S,\lambda V,\lambda\vec{N})\,S-P(\lambda S,\lambda V,\lambda\vec{N})\,V
+\sum_{i=1}^r\mu_i(\lambda S,\lambda V,\lambda\vec{N})\,N_i=\tilde{U}(S,V,\vec{N}).
\]
Taking $\lambda=1$ gives \eqref{eq:euler-equation}, as desired. ///
\end{proof}

Remark: Equation \eqref{eq:euler-equation} is known as Euler's Equation.

\begin{definition}
\label{def:process-path}
\textup{(3.2)} A process path in state space $\Sigma_S$,
\[
\Sigma_S\subseteq [0,\infty)\times[0,\infty)\times[0,\infty)\times\cdots\times[0,\infty),
\]
is a continuous, piecewise differentiable function $\vec{Y}:[0,1]\to\Sigma_S$, defined by
\[
\vec{Y}(\gamma)=
\begin{bmatrix}
S(\gamma)\\
V(\gamma)\\
N_1(\gamma)\\
\vdots\\
N_r(\gamma)
\end{bmatrix}.
\]
A process path in $\Sigma_U$ is defined similarly.
\end{definition}

Thus, using the chain rule, we have
\begin{align}
\frac{d}{d\gamma}\tilde{U}\big(\vec{Y}(\gamma)\big)
&=T\big(\vec{Y}(\gamma)\big)S'(\gamma)-P\big(\vec{Y}(\gamma)\big)V'(\gamma)
+\sum_{i=1}^r\mu_i\big(\vec{Y}(\gamma)\big)N_i'(\gamma)
\tag{3.5}\label{eq:chain-rule-u}
\end{align}
for a valid process path in state space.

\begin{theorem}
\label{thm:gibbs-duhem}
\textup{(3.3)} Suppose that $\vec{Y}:[0,1]\to\Sigma_S$ is a process path in state space $\Sigma_S$. Then
\begin{equation}
0=S(\gamma)\frac{dT_S(\vec{Y}(\gamma))}{d\gamma}-V(\gamma)\frac{dP_S(\vec{Y}(\gamma))}{d\gamma}
+\sum_{i=1}^r N_i(\gamma)\frac{d\mu_S^i(\vec{Y}(\gamma))}{d\gamma}.
\tag{3.6}\label{eq:gibbs-duhem}
\end{equation}
This equation is called the Gibbs-Duhem relation.
\end{theorem}

\begin{proof}
Begin with the Euler equation and differentiate with respect to the process parameter $\gamma$:
\begin{align}
\frac{d\tilde{U}}{d\gamma}\big(\vec{Y}(\gamma)\big)
&=\frac{dT}{d\gamma}\big(\vec{Y}(\gamma)\big)S(\gamma)+T\big(\vec{Y}(\gamma)\big)S'(\gamma) \notag \\
&\quad -\frac{dP}{d\gamma}\big(\vec{Y}(\gamma)\big)V(\gamma)-P\big(\vec{Y}(\gamma)\big)V'(\gamma) \notag \\
&\quad +\sum_{i=1}^r\left\{\frac{d\mu_i}{d\gamma}\big(\vec{Y}(\gamma)\big)N_i(\gamma)
+\mu_i\big(\vec{Y}(\gamma)\big)N_i'(\gamma)\right\}.
\tag{3.7}\label{eq:euler-derivative}
\end{align}
Substituting \eqref{eq:chain-rule-u} into \eqref{eq:euler-derivative} yields \eqref{eq:gibbs-duhem}. ///
\end{proof}

\THERMOEND
