\newif\ifthermosubfile
\ifdefined\THERMONOTESMAIN
  \thermosubfilefalse
\else
  \thermosubfiletrue
\fi

\providecommand{\THERMOEND}{} % safe in both modes

\ifthermosubfile
  \documentclass[11pt]{book}
  \input{./Macros/thermoHead}
  \input{./Macros/thermoSymbols}
  \graphicspath{{./Figures/}}
  \begin{document}
  \renewcommand{\THERMOEND}{\end{document}}
\fi


\chapter{ThermoS26-06}
\label{chap:ThermoS26-06}

\section{Legendre Transforms and Thermodynamic Potentials}

\begin{definition}
\label{def:legendre}
\textup{(5.1)} Suppose that $f:[a,b]\to\mathbb{R}$ is
continuous. For every $p\in[c,d]$, define
\begin{equation}
f^\ast(p):=\sup_{x\in[a,b]}\{xp-f(x)\}
\tag{5.1}\label{eq:legendre-def}
\end{equation}
The function $f^\ast:[c,d]\to\mathbb{R}$ is called the
Legendre transform of $f$.
\end{definition}

\begin{theorem}
\label{thm:legendre-form}
\textup{(5.2)} Suppose that $f\in C^2([0,\infty);\mathbb{R})$
with
\[
f''(x)>0,\qquad\forall x\in[0,\infty).
\]
Then, for all $p\in\mathrm{Range}(f')$,
\begin{equation}
f^\ast(p)=x_p\,p-f(x_p),
\tag{5.2}\label{eq:legendre-form}
\end{equation}
where $x_p\in[0,\infty)$ is the unique solution to
\[
f'(x_p)=p.
\]
\end{theorem}

\begin{proof}
let $p\in\mathrm{Range}(f')$.
\[
f':[0,\infty)\to\mathrm{Range}(f')
\]
For every $p\in\mathrm{Range}(f')\ \exists!\ x_p\in[0,\infty)$ and that,
\[
f'(x_p)=p.
\]

Since $f':[0,\infty)$ is strictly increasing,

Fix $p\in\mathrm{Range}(f')$. By Taylor's Theorem,
\[
f(x)=f(x_p)+p(x-x_p)+\frac{1}{2}f''(\xi_p)(x-x_p)^2
\]
for some $\xi_p$ between $x$ and $x_p$.

\[
\sup_{0\le x<\infty}\{x\cdot p-f(x)\}
=\sup_{0\le x<\infty}\{x_p\cdot p-f(x_p)-\tfrac{1}{2}f''(\xi_p)(x-x_p)^2\}
\]
\[
= x_p\cdot p-f(x_p). ///
\]
\end{proof}

\begin{theorem}
\label{thm:legendre-derivs}
\textup{(5.3)} Suppose that $f\in C^2([0,\infty);\mathbb{R})$
with
\[
f''(x)>0,\qquad\forall x\in[0,\infty).
\]
Then,
\[
[f^\ast]'(p)=[f']^{-1}(p),\qquad [f^\ast]''(p)>0,
\]
for all $p\in\mathrm{Range}(f')$.
\end{theorem}

\begin{proof}
Recall
\[
f':[0,\infty)\to\mathrm{Range}(f')
\]

Then
\[
f'\big([f']^{-1}(p)\big)=p,\qquad\forall\ p\in\mathrm{Range}(f').
\]

Also, observe that $\frac{d}{dp}[f']^{-1}\in C(\mathrm{Range}(f');\mathbb{R}).$

Now,
\begin{align*}
\frac{d}{dp}[f^\ast(p)]&=\frac{d}{dp}\{x_p\cdot p-f(x_p)\}
=\frac{d}{dp}\{[f']^{-1}(p)\cdot p-f([f']^{-1}(p))\}\\
&=p\cdot\frac{d}{dp}[f']^{-1}(p)+[f']^{-1}(p)
-\frac{df}{dx}([f']^{-1}(p))\cdot\frac{d}{dp}[f']^{-1}(p)\\
&=[f']^{-1}(p).
\end{align*}

Now that this is established, we have
\[
\frac{d^2}{dp^2}[f^\ast(p)]=\frac{d}{dp}[f']^{-1}(p)
\]

for all $p\in\mathrm{Range}(f')$. Since $f''\in C([0,\infty))$ and
$f''(x)>0,\ \forall x\in[0,\infty)$,
\[
\frac{d}{dp}[f']^{-1}(p)>0,\qquad\forall p\in\mathrm{Range}(f'). ///
\]
\end{proof}

Finally, we observe the following:

\begin{theorem}
\label{thm:legendre-involution}
\textup{(5.4)} Suppose that $f\in C^2([0,\infty);\mathbb{R})$
with
\[
f''(x)>0,\qquad\forall x\in[0,\infty).
\]

Then $f^\ast\in C^2(\mathrm{Range}(f');\mathbb{R})$ with
\[
[f^\ast]''(p)>0,\qquad\forall p\in\mathrm{Range}(f')
\]

Furthermore
\begin{equation}
[f^\ast]^\ast(x)=f(x),\qquad\forall x\in[0,\infty).
\tag{5.3}\label{eq:legendre-involution}
\end{equation}

In other words, the Legendre transform is involutive
and in fact an isomorphism.
\end{theorem}

\begin{proof}
It follows that, for all $x\in[0,\infty)$,
\[
[f^\ast]^\ast(x)=x\,p_x-f^\ast(p_x),
\]

where $p_x\in\mathrm{Range}(f')$ is the unique solution to
\[
f^\ast{}'(p_x)=x.
\]

Recall
\[
f^\ast(p_x)=p_x\cdot x_{p_x}-f(x_{p_x}),
\]

where $x_{p_x}\in[0,\infty)$ is the unique solution to
\[
f'(x_{p_x})=p_x.
\]

Of course, by uniqueness,
\[
x_{p_x}=x.
\]

So,
\[
[f^\ast]^\ast(x)=x\cdot p_x-\{p_x\cdot x_{p_x}-f(x_{p_x})\}
=f(x). ///
\]
\end{proof}

Why is the Legendre transform useful in
Thermodynamics?

This transform allows us to introduce new
thermodynamics coordinates/variables.

Recall
\[
\tilde{U}=\tilde{U}(S,V,N)
\]

or
\[
 d\tilde{U}=T\,dS-p\,dV+\mu\,dN
\]

The latter means
\[
T=\frac{\partial \tilde{U}}{\partial S}\quad p=-\frac{\partial \tilde{U}}{\partial V}\quad \mu=\frac{\partial \tilde{U}}{\partial N}
\]

in short hand
\begin{table}[h]
\centering
\begin{tabular}{lll}
\toprule
Extensive Quantity & Conjugate Variable & Variable \\
\midrule
$\tilde{U}$ & $T,\,-p,\,\mu$ & $S,\,V,\,N$ \\
$\tilde{S}$ & $\frac{1}{T},\,\frac{p}{T},\,-\frac{\mu}{T}$ & $U,\,V,\,N$ \\
\bottomrule
\end{tabular}
\caption{Conjugate variables for $\tilde{U}$ and $\tilde{S}$.}
\label{tab:thermos26-05-conjugate-us}
\end{table}

\begin{definition}
\label{def:helmholtz}
\textup{(5.5)} Suppose that all of the
Thermodynamic Postulates hold. Assume that
the material in question is unary ($r=1$). Define
\begin{equation}
\tilde{F}(T,V,N)=\tilde{U}(S_T,V,N)-TS_T
\tag{5.4}\label{eq:helmholtz-def}
\end{equation}
where $S_T=S_T(V,N)$ is the unique solution of the
equation
\begin{equation}
T_U(S_T(V,N),V,N)=T
\tag{5.5}\label{eq:helmholtz-st}
\end{equation}
for fixed values of $N$ and $V$.

$\tilde{F}$ is called the Helmholtz free energy.

Formally, we have
\begin{align*}
 d\tilde{F}&=d\tilde{U}-S\,dT-T\,dS\\
&=T\,dS-p\,dV+\mu\,dN-S\,dT-T\,dS\\
&=-S\,dT-p\,dV+\mu\,dN.
\end{align*}

\begin{table}[h]
\centering
\begin{tabular}{lll}
\toprule
Extensive Quantity & Conjugate Variable & Variable \\
\midrule
$\tilde{U}$ & $T,\,-p,\,\mu$ & $S,\,V,\,N$ \\
$\tilde{F}$ & $-S,\,-p,\,\mu$ & $T,\,V,\,N$ \\
\bottomrule
\end{tabular}
\caption{Conjugate variables for $\tilde{U}$ and $\tilde{F}$.}
\label{tab:thermos26-05-conjugate-uf}
\end{table}
\end{definition}

\begin{example}
\label{ex:helmholtz-example}
\textup{(5.6)} Suppose that
\[
\tilde{S}(U,V,N)=\left(\frac{NVUR^2}{v_0\theta}\right)^{1/3}.
\]

It follows that
\[
\tilde{U}(S,V,N)=\frac{S^3 v_0\theta}{NVR^2}.
\]

The temperature function is
\[
T_U(S,V,N)=\frac{3S^2 v_0\theta}{NVR^2}.
\]

Or
\[
\frac{1}{T_S(U,V,N)}=\frac{1}{3}\left(\frac{NVUR^2}{v_0\theta}\right)^{-2/3}\frac{NV R^2}{v_0\theta}
=\frac{1}{3}\left(\frac{NV R^2}{v_0\theta}\right)^{1/3}U^{-2/3}.
\]

Thus
\[
T_S(U,V,N)=3\left(\frac{v_0\theta}{NVR^2}\right)^{1/3}U^{2/3}.
\]

Recall that
\[
T_U(S,V,\vec{N})=T_S(\tilde{U}(S,V,\vec{N}),V,\vec{N})
\]

\[
T_S(U,V,\vec{N})=T_U(\tilde{S}(U,V,\vec{N}),V,\vec{N}).
\]

By definition
\[
\tilde{F}(T,V,N)=\tilde{U}(S_T,V,N)-TS_T
\]

where

\[
T_U(S_T(V,N),V,N)=T.
\]

For our example,
\[
T_U(S,V,N)=\frac{3S^2 v_0\theta}{NVR^2}.
\]

Hence,
\[
S_T=\sqrt{\frac{TNV R^2}{3v_0\theta}}.
\]

Thus,
\begin{align*}
\tilde{F}(T,V,N)&=\tilde{U}\left(\sqrt{\frac{TNV R^2}{3v_0\theta}},V,N\right)
-T\sqrt{\frac{TNV R^2}{3v_0\theta}}\\
&=\left(\frac{TNV R^2}{3v_0\theta}\right)^{3/2}\frac{v_0\theta}{NVR^2}
-T\sqrt{\frac{TNV R^2}{3v_0\theta}}.
\end{align*}

But
\[
\tilde{U}(S_T,V,N)=\frac{S_T^3 v_0\theta}{NVR^2}
=\left(\frac{TNV R^2}{3v_0\theta}\right)^{3/2}\frac{v_0\theta}{NVR^2}
\]

so that
\[
\tilde{F}(T,N,V)=\frac{1}{3}T^{3/2}\frac{1}{\sqrt{3}}\sqrt{\frac{NV R^2}{v_0\theta}}
-\frac{T^{3/2}}{\sqrt{3}}\sqrt{\frac{NV R^2}{v_0\theta}}.
\]
\end{example}

Finally,
\begin{equation}
\tilde{F}(T,N,V)=-\frac{2T^{3/2}}{3}\sqrt{\frac{NV R^2}{3v_0\theta}}.
\tag{5.6}\label{eq:helmholtz-final}
\end{equation}

Now,
\[
\frac{\partial \tilde{F}}{\partial T}=-\frac{2}{3}\frac{3}{2}\sqrt{T}\,\sqrt{\frac{NV R^2}{3v_0\theta}}.
\]

But
\[
T_U(S,V,N)=\frac{3S^2 v_0\theta}{NVR^2}
\]

Thus,
\[
\sqrt{T}=\sqrt{\frac{3v_0\theta}{NVR^2}}\,S_T
\]

and
\begin{equation}
\frac{\partial \tilde{F}}{\partial T}=-S_T.
\tag{5.7}\label{eq:helmholtz-deriv}
\end{equation}

\begin{theorem}
\label{thm:helmholtz-proc}
\textup{(5.7)} Suppose that all of the
Thermodynamic Postulates hold. Assume that
the material in question is unary ($r=1$). The
following procedure is equivalent means for finding
the Helmholtz free energy:
\begin{equation}
\tilde{F}(T,V,N)=U_T-T\tilde{S}(U_T,V,N)
\tag{5.8}\label{eq:helmholtz-proc}
\end{equation}
\end{theorem}

where $U_T=U_T(V,N)$ is the unique solution of the
equation
\[
T_S(U_T(V,N),V,N)=T
\]

for fixed values of $N$ and $V$.

Proof: Exercise ///

\begin{example}
\label{ex:ideal-gas-helmholtz}
\textup{(5.8)} Let us use the second version
to calculate the free energy for the monatomic
ideal gas. Recall,
\[
\tilde{S}(U,V,N)=Ns_0+NR\ln\left(\left(\frac{U}{U_0}\right)^{3/2}\left(\frac{V}{V_0}\right)\left(\frac{N}{N_0}\right)^{-5/2}\right),
\]
where $s_0,R,U_0,V_0,N_0$ are positive
constants.

Then
\[
\frac{\partial \tilde{S}}{\partial U}
=\frac{NR}{\left(\frac{U}{U_0}\right)^{3/2}}\cdot \frac{3}{2}\left(\frac{U}{U_0}\right)^{1/2}\frac{1}{U_0}
\]

\[
=\frac{3NR}{2U_0}\cdot \frac{U_0}{U}
=\frac{3NR}{2U}
\]

Thus
\[
T_S(U,V,N)=\frac{2}{3}\frac{U}{NR}
\]

and
\[
U_T=\frac{3NRT}{2}
\]

Therefore,
\begin{align*}
\tilde{F}(T,V,N)&=\frac{3NRT}{2}-TN s_0\\
&\phantom{=} -NR T\ln\left(\left(\frac{3NRT}{2U_0}\right)^{3/2}\left(\frac{V}{V_0}\right)\left(\frac{N}{N_0}\right)^{-5/2}\right)
\end{align*}

Define
\[
T_0:=\frac{2U_0}{3N_0R}.
\]

Then,
\begin{equation}
\tilde{F}(T,V,N)=\frac{3NRT}{2}-TN s_0
-NRT\ln\left(\left(\frac{T}{T_0}\right)^{3/2}\left(\frac{V}{V_0}\right)\left(\frac{N}{N_0}\right)^{-1}\right)
\tag{5.9}\label{eq:ideal-helmholtz}
\end{equation}
\end{example}


\THERMOEND
